# 矩阵解方程
方程组：
$$
\begin{cases}
3x + 2y  = 7 \\
-6x + 6y  = 6 \\
\end{cases}
$$
矩阵表示：
$$\left[
\begin{matrix} 
3 & 2 \\ 
-6 & 6 \\
\end{matrix} 
\right]
\ast 
\left[
\begin{matrix} 
x  \\ 
y  \\
\end{matrix} 
\right] =
\left[
\begin{matrix} 
7 \\ 
6 \\
\end{matrix} 
\right]
$$
令：
$$ 
A=
\left[
\begin{matrix} 
3 & 2 \\ 
-6 & 6 \\
\end{matrix} 
\right] ,
B=
\left[
\begin{matrix} 
7  \\ 
6  \\
\end{matrix} 
\right]
$$

则：
$$ 
\left[
\begin{matrix} 
x  \\ 
y  \\
\end{matrix} 
\right]= A ^{-1} \ast   B
$$
由矩阵的逆矩阵定律知道 ：
$$
A ^{-1} = \frac{1}{｜A｜} \ast  A^{*}
$$
定理：
$$
设A=
\left[
\begin{matrix} 
a & b  \\ 
c & d  \\
\end{matrix} 
\right] , 当｜A｜= ad-bc \neq 0时，有
$$
$$
A ^{-1} = \frac{1}{｜A｜} \ast  A^{*} = \frac{1}{ad-bc}\ast 
\left[
\begin{matrix} 
d & {-b}  \\ 
{-c} & a  \\
\end{matrix}
\right]
$$
可得到：
$$
A ^{-1} = \frac{1}{30}
\ast 
\left[
\begin{matrix} 
6 & -2  \\ 
6 & 3  \\
\end{matrix}
\right]
$$
则得到方程的解为：
$$
\left[
\begin{matrix} 
x  \\ 
y  \\
\end{matrix} 
\right] =  \frac{1}{30}
\ast
\left[
\begin{matrix} 
6 & -2  \\ 
6 & 3  \\
\end{matrix}
\right] 
\ast
\left[
\begin{matrix} 
7  \\ 
6  \\
\end{matrix} 
\right] =
\frac{1}{30}
\ast 
\left[
\begin{matrix} 
30  \\ 
60  \\
\end{matrix} 
\right] =
\left[
\begin{matrix} 
1  \\ 
2  \\
\end{matrix} 
\right] 
$$
$$
\begin{cases}
x  = {1} \\ y  = {2} \\
\end{cases}
$$
### 参考链接
[原文连接](https://blog.csdn.net/qq_21476953/article/details/111896974)
[矩阵的逆的](https://www.sohu.com/a/226465524_224832)
[矩阵的乘法](https://jingyan.baidu.com/article/4ae03de3d2b8c13eff9e6b1e.html)
[矩阵的逆矩阵](https://jingyan.baidu.com/article/925f8cb8a74919c0dde056e7.html)
[Markdown数学公式表示](https://zhenkai.blog.csdn.net/article/details/88621318)
[Markdown数学公式](http://liyangbit.com/math/jupyter-latex/)